Removed strings from imp

imp/Imp/Expr/Basic.lean
@@ -11,15 +11,13 @@ inductive BinOp where
   | plus | minus | times | div
   | and | or
   | lt | le | eq
-  | append
 deriving Repr, DecidableEq
 
 end Expr
 
 /-- Expressions -/
 inductive Expr where
-  | constInt (i : Int)
-  | constStr (x : String)
+  | const (i : Int)
   | var (name : String)
   | un (op : Expr.UnOp) (e : Expr)
   | bin (op : Expr.BinOp) (e1 e2 : Expr)
